src/Stringification/IR.v
@@ -747,6 +747,7 @@ Module Compilers.
                  | ident.Nat_eqb
                  | ident.prod_rect _ _ _
                  | ident.bool_rect _
+                 | ident.bool_rect_nodep _
                  | ident.nat_rect _
                  | ident.eager_nat_rect _
                  | ident.nat_rect_arrow _ _
